Almost work.

src/QuickCodes.fst
@@ -5,21 +5,69 @@ open State
 open QuickCode
 open FStar.List
 
+(** * Comparing [reglist] *)
+
 let rec regs_list_match (#t:reg_t) (regs: list (regtyp t)) (r0:regmap) (r1:regmap) : Type0 =
 match regs with
 | [] -> True
 | r::regs' -> r0 t r == r1 t r /\ regs_list_match regs' r0 r1
 
+unfold
+let reglist_match (t:reg_t)(r0:regmap)(r1:regmap) : Type0 =
+	regs_list_match (reglist t) r0 r1
+
+(** * Lemmas about comparing [reglist] *)
+
+val lemma_regs_list_match : #t:reg_t -> regs:list (regtyp t) -> r0:regmap -> r1:regmap -> Lemma
+	(regs_list_match regs r0 r1 ==>
+	 (forall (r:regtyp t). mem r regs ==> r0 t r == r1 t r))
+let rec lemma_regs_list_match #t regs r0 r1 = 
+match regs with
+| [] -> ()
+| r::regs' -> lemma_regs_list_match regs' r0 r1
+
+val lemma_reglist_match : t:reg_t -> r0:regmap -> r1:regmap -> Lemma
+	(reglist_match t r0 r1 ==>
+	 r0 t == r1 t)
+let lemma_reglist_match t r0 r1 = 
+	lemma_regs_list_match (reglist t) r0 r1;
+	lemma_reglist_derive (fun r -> r0 t r == r1 t r);
+	assert (reglist_match t r0 r1 ==> equal1 (r0 t) (r1 t))
+
+(** * Comparing [regclasses] *)
+
 let rec regs_class_match (regs: list reg_t) (r0:regmap) (r1:regmap) : Type0 =
 match regs with
 | [] -> True
-| t::regs' -> regs_list_match (reglist t) r0 r1 /\ regs_class_match regs' r0 r1
+| t::regs' -> reglist_match t r0 r1 /\ regs_class_match regs' r0 r1
 
-let regs_match (r0:regmap) (r1:regmap) : Type0 =
-  regs_class_match regclasses r0 r1
+unfold 
+let regclasses_match (r0:regmap) (r1:regmap) : Type0 =
+	regs_class_match regclasses r0 r1
+
+(** * Lemmas about comparing [regclasses] *)
+
+val lemma_regs_class_match : regs:(list reg_t) -> r0:regmap -> r1:regmap -> Lemma
+	(regs_class_match regs r0 r1 ==>
+	 (forall t. mem t regs ==> r0 t == r1 t))
+let rec lemma_regs_class_match regs r0 r1 =
+match regs with
+| [] -> ()
+| t::regs' -> lemma_reglist_match t r0 r1; lemma_regs_class_match regs' r0 r1
+
+val lemma_regclasses_match : r0:regmap -> r1:regmap -> Lemma
+	(regclasses_match r0 r1 ==>
+	 r0 == r1)
+let rec lemma_regclasses_match r0 r1 =
+	lemma_regs_class_match regclasses r0 r1;
+	lemma_regclasses_derive (fun t -> r0 t == r1 t);
+	assert (regclasses_match r0 r1 ==> equal r0 r1)
+
+(** [va_state_match] *)
 
 let va_state_match (s0:state) (s1:state) : Pure Type0
     (requires True)
     (ensures fun b -> b ==> state_eq s0 s1) =
+	let _ = lemma_regclasses_match s0.regs s1.regs in
     s0.ok == s1.ok /\
-    regs_match s0.regs s1.regs
+    regclasses_match s0.regs s1.regs
