src/Regs.fst
@@ -2,54 +2,20 @@ module Regs
 
 open FStar.FunctionalExtensionality
 
-type reg_t = n:int{0 <= n /\ n <= 1}
+let n_reg_t : n:nat{0 < n} = 2
 
-type reg =
-  | Rax
-  | Rbx
-  | Rcx
-  | Rdx
-  | Rsi
-  | Rdi
-  | Rbp
-  | Rsp
-  | R8
-  | R9
-  | R10
-  | R11
-  | R12
-  | R13
-  | R14
-  | R15
+let n_regtype _ : n:nat{0 < n} = 16
 
-let list_reg = [Rax; Rbx; Rcx; Rdx; Rsi; Rdi; Rbp; Rsp; R8; R9; R10; R11; R12; R13; R14; R15]
+let regval _ = nat
 
-type xmm = i:int{ 0 <= i /\ i < 16 }
+let equal1 #_ f1 f2 = feq f1 f2
 
-let list_xmm : list xmm = [0; 1; 2; 3; 4; 5; 6; 7; 8; 9; 10; 11; 12; 13; 14; 15]
+let equal f1 f2 = forall t. equal1 (f1 t) (f2 t)
 
-let regtyp (t:reg_t) : Type =
-  match t with
-  | 0 -> reg
-  | 1 -> xmm
+let lemma_equal1_intro t regs1 regs2 = ()
 
-(* wrong definition, use for convenience right now *)
-type nat32=n:int{0 <= n /\ n < 32}
-type nat64=n:int{0 <= n /\ n < 64}
-type quad32=(nat32 * nat32 * nat32 * nat32)
+let lemma_equal1_elim t regs1 regs2 = ()
 
-let regval t =
-  match t with
-  | 0 -> nat64
-  | 1 -> quad32
-
-let reglist t =
-  match t with
-  | 0 -> list_reg
-  | 1 -> list_xmm
-
-let regclasses = [0; 1]
-
-let equal regs1 regs2 = feq regs1 regs2
 let lemma_equal_intro regs1 regs2 = ()
+
 let lemma_equal_elim regs1 regs2 = ()
