src/Regs.fsti
@@ -1,42 +1,56 @@
 module Regs
 
 open FStar.List
+open Util
 
-val reg_t : eqtype
+val n_reg_t : n:nat{0 < n}
 
-val regtyp : reg_t -> eqtype
+type reg_t = n:nat{n < n_reg_t}
 
-val regval : reg_t -> eqtype
+let regclasses : list reg_t = range n_reg_t
 
-val reglist : t:reg_t -> list (regtyp t)
+let lemma_regclasses_complete : unit -> Lemma
+	(forall (t:reg_t). mem t regclasses) = fun _ ->
+	lemma_range_complete n_reg_t;
+	assert (forall (t:reg_t). t < n_reg_t)
 
-val regclasses : list (reg_t)
+let lemma_regclasses_derive : p:(reg_t -> Type0) -> Lemma
+	((forall t0. mem t0 regclasses ==> p t0) ==> (forall t. p t)) = fun _ ->
+	lemma_regclasses_complete ()
+
+val n_regtype : reg_t -> n:nat{0 < n}
+
+unfold type regtyp (t:reg_t) = n:nat{n < n_regtype t}
+
+(* why [list (regtyp t)] does not work here? *)
+let reglist (t:reg_t) : list (regtyp t) = range (n_regtype t)
+
+let lemma_reglist_complete : t:reg_t -> Lemma
+	(forall r. mem r (reglist t)) = fun t ->
+	lemma_range_complete (n_regtype t)
+
+let lemma_reglist_derive : #t:reg_t -> p:(regtyp t -> Type0) -> Lemma
+	((forall r0. mem r0 (reglist t) ==> p r0) ==> (forall r. p r)) = fun #t p ->
+	lemma_reglist_complete t
+
+val regval : reg_t -> Type0
+
 
 type regmap = t:reg_t -> regtyp t -> regval t
 
+val equal1 : #t:reg_t -> (regtyp t -> regval t) -> (regtyp t -> regval t) -> Type0
+
 val equal : regmap -> regmap -> Type0
-
-val equal1 : t:reg_t -> (regtyp t -> regval t) -> (regtyp t -> regval t) -> Type0
-
-val lemma_reglist_complete (t:reg_t) : r:regtyp t -> Lemma
-  (requires True)
-  (ensures mem r (reglist t) == true)
-  [SMTPat (mem r (reglist t) == true)]
-
-val lemma_regclasses_complete : t:reg_t -> Lemma
-  (requires True)
-  (ensures mem t regclasses == true)
-  [SMTPat (mem t regclasses == true)]
 
 val lemma_equal1_intro : t:reg_t -> regs1:regmap -> regs2:regmap -> Lemma
   (requires forall r. regs1 t r == regs2 t r)
-  (ensures equal1 t (regs1 t) (regs2 t))
-  [SMTPat (equal1 t (regs1 t) (regs2 t))]
+  (ensures equal1 (regs1 t) (regs2 t))
+  [SMTPat (equal1 (regs1 t) (regs2 t))]
 
 val lemma_equal1_elim : t:reg_t -> regs1:regmap -> regs2:regmap -> Lemma
-  (requires equal1 t (regs1 t) (regs2 t))
+  (requires equal1 (regs1 t) (regs2 t))
   (ensures regs1 t == regs2 t)
-  [SMTPat (equal1 t (regs1 t) (regs2 t))]
+  [SMTPat (equal1 (regs1 t) (regs2 t))]
 
 val lemma_equal_intro : regs1:regmap -> regs2:regmap -> Lemma
   (requires forall t. regs1 t == regs2 t)
