src/Util.fst
@@ -1,0 +1,10 @@
+module Util
+
+let range (n:nat) : list (m:nat{m < n}) =
+	let rec range' (n':nat{n'<=n}) : list (m:nat{m < n}) =
+		if n' = 0 then [] else (n'-1) :: range' (n'-1) in
+	range' n
+
+let rec range_complete : n:nat -> Lemma
+	(forall m. m < n <==> mem m (range n)) =
+	fun n -> if n = 0 then () else range_complete (n-1)
