src/Util.fsti
@@ -1,0 +1,8 @@
+module Util
+
+open FStar.List
+
+val range : n:nat -> list (m:nat{m < n})
+
+val lemma_range_complete : n:nat -> Lemma
+	(forall m. m < n <==> mem m (range n))
