Makefile
@@ -1,2 +1,3 @@
 all:
 	fstar.exe src/QuickCodes.fst --include src --log_queries --record_hints
+	fstar.exe src/Regs.fst --include src --log_queries --record_hints
